mppa_k1c/Asmblockdeps.v
@@ -633,7 +633,7 @@ Fixpoint trans_body (b: list basic) : list L.inst :=
 
 Definition trans_pcincr (sz: Z) (k: L.inst) := (#PC, Op (Control (OIncremPC sz)) (PReg(#PC) @ Enil)) :: k.
 
-Definition trans_block (b: Asmblock.bblock) : L.bblock :=
+Definition trans_block (b: Asmvliw.bblock) : L.bblock :=
   trans_body (body b) ++ (trans_pcincr (size b) (trans_exit (exit b)) :: nil).
 
 Theorem trans_block_noheader_inv: forall bb, trans_block (no_header bb) = trans_block bb.
@@ -649,7 +649,7 @@ Qed.
 Definition state := L.mem.
 Definition exec := L.run.
 
-Definition match_states (s: Asmblock.state) (s': state) :=
+Definition match_states (s: Asmvliw.state) (s': state) :=
   let (rs, m) := s in
      s' pmem = Memstate m
   /\ forall r, s' (#r) = Val (rs r).
@@ -662,7 +662,7 @@ Definition match_outcome (o:outcome) (s: option state) :=
  
 Notation "a <[ b <- c ]>" := (assign a b c) (at level 102, right associativity).
 
-Definition trans_state (s: Asmblock.state) : state :=
+Definition trans_state (s: Asmvliw.state) : state :=
   let (rs, m) := s in
   fun x => if (Pos.eq_dec x pmem) then Memstate m
            else match (inv_ppos x) with
@@ -1537,7 +1537,7 @@ Definition string_of_op (op: P.op): ?? pstring :=
   | Fail => RET (Str "Fail")
   end.
 
-Definition bblock_eq_test (verb: bool) (p1 p2: Asmblock.bblock) : ?? bool :=
+Definition bblock_eq_test (verb: bool) (p1 p2: Asmvliw.bblock) : ?? bool :=
   if verb then
     IDT.verb_bblock_eq_test string_of_name string_of_op (trans_block p1) (trans_block p2)
   else
@@ -1556,7 +1556,7 @@ Hint Resolve bblock_eq_test_correct: wlp.
 
 Import UnsafeImpure.
 
-Definition pure_bblock_eq_test (verb: bool) (p1 p2: Asmblock.bblock): bool := unsafe_coerce (bblock_eq_test verb p1 p2).
+Definition pure_bblock_eq_test (verb: bool) (p1 p2: Asmvliw.bblock): bool := unsafe_coerce (bblock_eq_test verb p1 p2).
 
 Theorem pure_bblock_eq_test_correct verb p1 p2:
   forall ge fn, Ge = Genv ge fn ->
@@ -1566,7 +1566,7 @@ Proof.
    apply unsafe_coerce_not_really_correct; eauto.
 Qed.
 
-Definition bblock_equivb: Asmblock.bblock -> Asmblock.bblock -> bool := pure_bblock_eq_test true.
+Definition bblock_equivb: Asmvliw.bblock -> Asmvliw.bblock -> bool := pure_bblock_eq_test true.
 
 Definition bblock_equiv_eq := pure_bblock_eq_test_correct true.
 
@@ -1576,7 +1576,7 @@ End SECT.
 
 Module PChk := ParallelChecks L PosPseudoRegSet.
 
-Definition bblock_para_check (p: Asmblock.bblock) : bool :=
+Definition bblock_para_check (p: Asmvliw.bblock) : bool :=
   PChk.is_parallelizable (trans_block p).
 
 Require Import Asmvliw Permutation.
